src/impl/TLS13.Impl.Client.fsti
@@ -86,6 +86,8 @@ let next_local_action_sound
       st.CS.cs_model.CS.model_control ==
         CS.ControlHandshaking CS.HsServerFinishedReceived /\
       Some? st.CS.cs_model.CS.model_handshake.CS.hs_server_finished /\
+      Some?
+        st.CS.cs_model.CS.model_handshake.CS.hs_keys.CS.ks_server_handshake_traffic /\
       st.CS.cs_model.CS.model_handshake.CS.hs_server_finished_verified == false /\
       B.length st.CS.cs_model.CS.model_handshake.CS.hs_transcript +
         SZ.v server_finished_payload_len <= C.max_transcript_len
