src/impl/TLS13.Impl.Handle.Local.fst
@@ -868,71 +868,105 @@ fn handle_local_event
     LocalVerifyFinished -> {
     let ready = C.can_verify_server_finished c payload_len;
     if ready {
-      let fin = Ghost.hide (Some?.v 'st0.CS.cs_model.CS.model_handshake.CS.hs_server_finished);
-      assert (pure ('st0.CS.cs_model.CS.model_handshake.CS.hs_server_finished ==
-        Some (Ghost.reveal fin)));
-      assert (pure (CT.local_input_wf
-        'st0
-        CT.LocalVerifyFinished
-        (Ghost.reveal 'payload_bytes)));
-      assert (pure ('st0.CS.cs_model.CS.model_control ==
-        CS.ControlHandshaking CS.HsServerFinishedReceived));
-      assert (pure (CS.legal_event
-        'st0.CS.cs_model
-        (CS.ConnLocalEvent
-          (CS.LocalVerifyFinished (Ghost.reveal fin)))));
-      assert (pure (Seq.equal
-        (Ghost.reveal 'payload_bytes)
-        (TLS13.Wire.Spec.serialize_handshake (TLS13.Messages.Finished (Ghost.reveal fin)))));
-      C.mark_verified_server_finished c payload payload_len #fin;
-      let resp = {
-        CT.network_out_len = 0sz;
-        CT.app_out_len = 0sz;
-        CT.status = CT.StepOk;
-      };
-      Seq.lemma_len_slice 'old_network_out 0 0;
-      Seq.lemma_eq_intro B.empty (Seq.slice 'old_network_out 0 0);
-      assert (pure (Seq.equal B.empty (CT.response_network_out resp 'old_network_out)));
-      C.lemma_verified_server_finished_state_evolves
-        'st0
-        (Ghost.reveal fin);
-      assert (pure (CT.legal_response_for_event
-        'st0
-        (C.verified_server_finished_state 'st0 (Ghost.reveal fin))
+      let finished_ok = C.server_finished_verify_data_matches c;
+      if finished_ok {
+        let fin = Ghost.hide (Some?.v 'st0.CS.cs_model.CS.model_handshake.CS.hs_server_finished);
+        assert (pure ('st0.CS.cs_model.CS.model_handshake.CS.hs_server_finished ==
+          Some (Ghost.reveal fin)));
+        assert (pure (CT.local_input_wf
+          'st0
+          CT.LocalVerifyFinished
+          (Ghost.reveal 'payload_bytes)));
+        assert (pure ('st0.CS.cs_model.CS.model_control ==
+          CS.ControlHandshaking CS.HsServerFinishedReceived));
+        assert (pure (CS.legal_event
+          'st0.CS.cs_model
+          (CS.ConnLocalEvent
+            (CS.LocalVerifyFinished (Ghost.reveal fin)))));
+        assert (pure (Seq.equal
+          (Ghost.reveal 'payload_bytes)
+          (TLS13.Wire.Spec.serialize_handshake (TLS13.Messages.Finished (Ghost.reveal fin)))));
+        C.mark_verified_server_finished c payload payload_len #fin;
+        let resp = {
+          CT.network_out_len = 0sz;
+          CT.app_out_len = 0sz;
+          CT.status = CT.StepOk;
+        };
+        Seq.lemma_len_slice 'old_network_out 0 0;
+        Seq.lemma_eq_intro B.empty (Seq.slice 'old_network_out 0 0);
+        assert (pure (Seq.equal B.empty (CT.response_network_out resp 'old_network_out)));
+        C.lemma_verified_server_finished_state_evolves
+          'st0
+          (Ghost.reveal fin);
+        assert (pure (CT.legal_response_for_event
+          'st0
+          (C.verified_server_finished_state 'st0 (Ghost.reveal fin))
+          resp
+          (CS.ConnLocalEvent
+            (CS.LocalVerifyFinished (Ghost.reveal fin)))
+          B.empty
+          B.empty
+          'old_network_out
+          'old_app_out));
+        assert (pure (CT.legal_local_response
+          'st0
+          (C.verified_server_finished_state 'st0 (Ghost.reveal fin))
+          resp
+          CT.LocalVerifyFinished
+          (Ghost.reveal 'payload_bytes)
+          (CS.ConnLocalEvent
+            (CS.LocalVerifyFinished (Ghost.reveal fin)))
+          B.empty
+          B.empty
+          'old_network_out
+          'old_app_out));
+        assert (pure (CT.legal_handled_local_response
+          'st0
+          (C.verified_server_finished_state 'st0 (Ghost.reveal fin))
+          resp
+          CT.LocalVerifyFinished
+          (Ghost.reveal 'payload_bytes)
+          'old_network_out
+          'old_app_out));
+        assert (pure (CT.some_legal_response
+          'st0
+          (C.verified_server_finished_state 'st0 (Ghost.reveal fin))
+          resp
+          'old_network_out
+          'old_app_out));
         resp
-        (CS.ConnLocalEvent
-          (CS.LocalVerifyFinished (Ghost.reveal fin)))
-        B.empty
-        B.empty
-        'old_network_out
-        'old_app_out));
-      assert (pure (CT.legal_local_response
-        'st0
-        (C.verified_server_finished_state 'st0 (Ghost.reveal fin))
+      } else {
+        C.mark_bad_finished c;
+        let resp = {
+          CT.network_out_len = 0sz;
+          CT.app_out_len = 0sz;
+          CT.status = CT.ConnectionFailed;
+        };
+        Seq.lemma_len_slice 'old_network_out 0 0;
+        Seq.lemma_eq_intro B.empty (Seq.slice 'old_network_out 0 0);
+        assert (pure (Seq.equal B.empty (CT.response_network_out resp 'old_network_out)));
+        assert (pure (CT.bad_finished_response
+          'st0
+          (C.local_fail_state 'st0 C.tls_bad_finished_error)
+          resp
+          'old_network_out
+          'old_app_out));
+        assert (pure (CT.legal_handled_local_response
+          'st0
+          (C.local_fail_state 'st0 C.tls_bad_finished_error)
+          resp
+          CT.LocalVerifyFinished
+          (Ghost.reveal 'payload_bytes)
+          'old_network_out
+          'old_app_out));
+        assert (pure (CT.some_legal_response
+          'st0
+          (C.local_fail_state 'st0 C.tls_bad_finished_error)
+          resp
+          'old_network_out
+          'old_app_out));
         resp
-        CT.LocalVerifyFinished
-        (Ghost.reveal 'payload_bytes)
-        (CS.ConnLocalEvent
-          (CS.LocalVerifyFinished (Ghost.reveal fin)))
-        B.empty
-        B.empty
-        'old_network_out
-        'old_app_out));
-      assert (pure (CT.legal_handled_local_response
-        'st0
-        (C.verified_server_finished_state 'st0 (Ghost.reveal fin))
-        resp
-        CT.LocalVerifyFinished
-        (Ghost.reveal 'payload_bytes)
-        'old_network_out
-        'old_app_out));
-      assert (pure (CT.some_legal_response
-        'st0
-        (C.verified_server_finished_state 'st0 (Ghost.reveal fin))
-        resp
-        'old_network_out
-        'old_app_out));
-      resp
+      }
     } else {
       C.mark_unexpected_message c;
       let resp = {
